examples/acl2/ml/translateLib.sig
@@ -1,0 +1,25 @@
+signature translateLib = 
+sig
+	include Abbrev
+
+	val CHOOSEP_TAC             : thm list -> tactic
+	val CHOOSEP		    : thm list -> term -> thm
+	val DOUBLE_MATCH            : (term -> term) -> (term -> term) -> term -> thm -> thm
+
+	val ite_tm                  : term
+	val mk_acl2_cond            : term * term * term -> term 
+	val dest_acl2_cond          : term -> term * term * term
+    	val is_acl2_cond            : term -> bool
+
+	val acl2_cons_tm            : term
+	val mk_acl2_cons            : term * term -> term
+	val dest_acl2_cons          : term -> term * term
+	val strip_cons              : term -> term list
+
+	val acl2_true_tm            : term
+	val mk_acl2_true            : term -> term
+	val dest_acl2_true          : term -> term
+	val is_acl2_true            : term -> bool
+	
+	val DISJ_CASES_UNIONL       : thm -> thm list -> thm
+end
