examples/acl2/ml/translateLib.sml
@@ -1,0 +1,149 @@
+(*****************************************************************************)
+(* File: translateLib.sml                                                    *)
+(* Author: James Reynolds                                                    *)
+(*                                                                           *)
+(* Provides tools to assist in proving theorems about translation between    *)
+(* s-expressions and native HOL                                              *)
+(*****************************************************************************)
+
+open Feedback Lib Type Term boolSyntax Thm Drule Tactical Thm_cont Tactic Conv;
+
+(*****************************************************************************)
+(* DOUBLE_MATCH: Like PART_MATCH but matches variables in the term as well   *)
+(*****************************************************************************)
+
+local
+	val match = mk_HOL_ERR "translateLib" "DOUBLE_MATCH" "Couldn't match terms"
+
+	fun inst_it a b = ((* print_term a ; print " --> " ; print_term b ; print "\n" ; *) inst (match_type (type_of a) (type_of b)))
+	
+	(* fun subst a = (app (fn {redex,residue} => (print_term redex ; print " |-> " ; print_term residue ; print "\n")) a ; Term.subst a); *)
+
+	(* Matches instantiating free variables to terms if possible, or instantiating t1 |-> t2 if not *)
+	fun tmatch (t1,t2) = 
+	case (strip_comb t1)
+	of (fx,x::xs) => (case (strip_comb t2)
+		of (fy,y::ys) => 
+			let 	val diff = length (y::ys) - length (x::xs)
+				val (fy',ys,fx',xs) = if 0 < diff 	then (list_mk_comb(fy,(List.take(y::ys,diff))),List.drop(y::ys,diff),fx,x::xs)
+									else (fy,y::ys,list_mk_comb(fx,(List.take(x::xs,~diff))),List.drop(x::xs,~diff))
+			in
+				(fn f' => foldl (fn (m,f) => tmatch ((f ## f) m) o f) f' (map (f' ## f') (zip xs ys)))
+				(if is_var fx' then 		(subst [inst_it fx' fy' fx' |-> fy'])
+				else (if same_const fx' fy' then 	I
+				else (if is_var fy' then 	(subst [inst_it fy' fx' fy' |-> fx'] o inst_it fy' fx') else raise match)))
+			end
+		| (fy,[]) => if is_var fy then subst [inst_it fy t1 fy |-> t1] o inst_it fy t1 else raise match)
+	| (fx,[]) => 
+		if is_var fx then (subst [inst_it fx t2 fx |-> t2])  else 
+			(if same_const fx t2 then I else (if is_var t2 then (subst [inst_it t2 fx t2 |-> fx] o inst_it t2 fx) else raise match))
+in
+	fun DOUBLE_MATCH opr1 opr2 term thm = 
+	let	val t1 = (opr1 o concl o SPEC_ALL) thm
+	in	PART_MATCH opr1 (SPEC_ALL thm) (tmatch (opr2 t1,opr2 term) term)
+	end
+end;
+
+
+(*****************************************************************************)
+(* CHOOSEP: Tactic to choose values if a predicate exists                    *)
+(*****************************************************************************)
+
+local
+	fun snd_to_last_imp term = case (strip_imp term) of ([],a) => a |  (xs,a) => last xs;
+	fun last_two_imps term = case (strip_imp term) of ([],a) => a | (xs,a) => mk_imp(last xs,a);
+	fun MATCH opr1 opr2 de_thms a = tryfind (DOUBLE_MATCH opr1 opr2 a o DISCH_ALL o SPEC_ALL o UNDISCH_ALL) de_thms
+	
+	fun fix_hyps de_thms thm = 
+	let	val hs = mapfilter (fn x => (x,(fn (a,b) => (GENL a o MATCH last_two_imps I de_thms) b) (strip_forall x)))  (filter is_forall (hyp thm))
+	in	if null hs then thm else fix_hyps de_thms 
+			(foldl (uncurry PROVE_HYP o (snd ## I)) (foldl (uncurry INST_TY_TERM) thm (map (uncurry match_term o (I ## concl)) hs)) hs)
+	end;
+	val sexp_to_term = rand o lhs o concl
+	val var = rhs o concl
+	fun exist L thm = 
+	let 	val new_var = if is_var (var thm) then mk_var(prime((fst o dest_var o var) thm),(type_of o sexp_to_term) thm) else 
+				variant (free_varsl L) (mk_var("x",(type_of o sexp_to_term) thm))
+	in	EXISTS (Psyntax.mk_exists(new_var,subst [sexp_to_term thm |-> new_var] (concl thm)),sexp_to_term thm) thm
+	end	
+in
+fun CHOOSEP decode_encode_thms x = 
+	DISCH_ALL (fix_hyps decode_encode_thms (MATCH_MP ((DISCH x o UNDISCH_ALL o MATCH snd_to_last_imp (rator o rand) decode_encode_thms) x) (ASSUME x)))
+fun CHOOSEP_TAC decode_encode_thms (assums,goal) = 
+	MAP_EVERY 
+		(CHOOSE_THEN SUBST_ALL_TAC o GSYM) 
+		(mapfilter (fn x => exist (goal::assums) 
+			(fix_hyps decode_encode_thms (MATCH_MP ((DISCH x o UNDISCH_ALL o MATCH snd_to_last_imp (rator o rand) decode_encode_thms) x) (ASSUME x)))) assums)
+		(assums,goal)
+end;
+
+(*****************************************************************************)
+(* DISJ_CASES_UNIONL: Like DISJ_CASES_UNION but with a list                  *)
+(*****************************************************************************)
+
+fun DISJ_CASES_UNIONL nchotomy thms = 
+let	val concls = map concl thms
+	fun make_or (n,t) =
+	let	val (pre,post) = (I ## tl) (split_after n concls);
+	in	foldl (uncurry DISJ2) (if not (null post) then DISJ1 t (list_mk_disj post) else t) (rev pre)
+	end
+in
+	DISJ_CASESL nchotomy (map make_or (enumerate 0 thms))
+end;
+	
+(*****************************************************************************)
+(* Some common destructors / constructors                                    *)
+(*****************************************************************************)
+
+fun raise_error a b = raise (mk_HOL_ERR "translateLib" a b)
+
+(* Create and destruct acl2_cond *)
+val ite_tm = ``ite``;
+
+fun mk_acl2_cond (p,a,b) = 
+	if not (type_of a = ``:sexp`` andalso type_of b = ``:sexp`` andalso type_of p = ``:sexp``) then raise_error "mk_acl2_cond" "Arguments not of type :sexp"
+	else mk_comb(mk_comb(mk_comb(ite_tm,p),a),b);
+
+fun dest_acl2_cond term = 
+    case strip_comb term
+     of (ite,[p,a,b]) =>
+         if same_const ite ite_tm
+         then (p,a,b)
+         else raise_error "dest_acl2_cond" "not an application of \"ite\""
+      | _ => raise_error "dest_acl2_cond" "not an application of \"ite\""
+
+fun is_acl2_cond term = 
+     case strip_comb term
+     of (ite,[p,a,b]) => same_const ite ite_tm | _ => false;
+
+
+(* Create and destruct acl2_cons *)
+val acl2_cons_tm = ``cons``;
+
+fun mk_acl2_cons (a,b) = 
+	if not (type_of a = ``:sexp`` andalso type_of b = ``:sexp``) then raise_error "mk_acl2_cons" "Arguments not of type :sexp"
+	else mk_comb(mk_comb(acl2_cons_tm,a),b);
+
+fun dest_acl2_cons term = 
+	case strip_comb term
+		of (acl2_cons,[a,b]) => if same_const acl2_cons acl2_cons_tm then (a,b) else raise_error "dest_acl2_cons" "not an application of \"cons\""
+		| _                  => raise_error "dest_acl2_cons" "not an application of \"cons\"";
+
+fun strip_cons term = 
+	case (strip_comb term)
+		of (a,[l,r]) => if same_const a ``cons`` then (strip_cons l) @ (strip_cons r) else [term]
+		 | _         => [term];
+
+(* Create and destruct acl2_true *)
+val acl2_true_tm = ``$|=``;
+
+val mk_acl2_true = curry mk_comb acl2_true_tm;
+
+fun dest_acl2_true term = 
+	case strip_comb term 
+	of (acl2_true,[a]) => if same_const acl2_true acl2_true_tm then a else raise_error "dest_acl2_true" "Not an application of \"|=\""
+	| _                => raise_error "dest_acl2_true" "Not an application of \"|=\"";
+
+fun is_acl2_true term = 
+	case strip_comb term of (acl2_true,[a]) => same_const acl2_true acl2_true_tm | _ => false;
+
